separate consistentS and R_

DP_Consistency.thy
@@ -1,125 +1,173 @@
 theory DP_Consistency
   imports "DP_Lifting"
 begin
-
+  
+locale dp_consistency =
+  fixes dp :: "'param \<Rightarrow> 'result"
+begin
+  
 context
   includes lifting_syntax
 begin
-
-(* Predicates *)
-definition consistentM :: "('param \<Rightarrow> 'result) \<Rightarrow> ('param \<rightharpoonup> 'result) \<Rightarrow> bool" where
-  "consistentM dp M \<equiv> \<forall>param\<in>dom M. M param = Some (dp param)"
+  
+  (* Predicates *)
+definition consistentM :: "('param \<rightharpoonup> 'result) \<Rightarrow> bool" where
+  "consistentM M \<equiv> \<forall>param\<in>dom M. M param = Some (dp param)"
 term 0 (**)
   
-definition consistentS :: "('param \<Rightarrow> 'result) \<Rightarrow> 'a \<Rightarrow> ('param \<rightharpoonup> 'result, 'a) state \<Rightarrow> bool" where
-  "consistentS dp v s \<equiv> \<forall>M. consistentM dp M \<longrightarrow> (case runState s M of (v', M') \<Rightarrow> v = v' \<and> consistentM dp M')"
+definition consistentS :: "('a \<Rightarrow> 'b \<Rightarrow> bool) \<Rightarrow> 'a \<Rightarrow> ('param \<rightharpoonup> 'result, 'b) state \<Rightarrow> bool" where
+  "consistentS R v s \<equiv> \<forall>M. consistentM M \<longrightarrow> (case runState s M of (v', M') \<Rightarrow> R v v' \<and> consistentM M')"
 term 0 (**)
-
-(* Consistency predicates for functions *)
-definition consistentS_0arg :: "('param \<Rightarrow> 'result) \<Rightarrow> 'a \<Rightarrow> ('param \<rightharpoonup> 'result, 'a) state \<Rightarrow> bool" where
-  "consistentS_0arg dp v v\<^sub>T \<equiv> consistentS dp v v\<^sub>T"
-definition consistentS_1arg :: "('param \<Rightarrow> 'result) \<Rightarrow> ('a \<Rightarrow> 'b) \<Rightarrow> ('param \<rightharpoonup> 'result, 'a ==_\<Longrightarrow> 'b) state \<Rightarrow> bool" where
-  "consistentS_1arg dp f f\<^sub>T \<equiv> \<forall>x. consistentS_0arg dp (f x) (f\<^sub>T . \<langle>x\<rangle>)"
-definition consistentS_2arg :: "('param \<Rightarrow> 'result) \<Rightarrow> ('a \<Rightarrow> 'b \<Rightarrow> 'c) \<Rightarrow> ('param \<rightharpoonup> 'result, 'a ==_\<Longrightarrow> 'b ==_\<Longrightarrow> 'c) state \<Rightarrow> bool" where
-  "consistentS_2arg dp f f\<^sub>T \<equiv> \<forall>x. consistentS_1arg dp (f x) (f\<^sub>T . \<langle>x\<rangle>)"
+  
+  (* Consistency predicates for functions *)
+abbreviation R_' :: "'a \<Rightarrow> 'a \<Rightarrow> bool" where
+  "R_' \<equiv> op ="
+abbreviation R_3 :: "('a \<Rightarrow> 'b) \<Rightarrow> ('a ==_\<Longrightarrow> 'b) \<Rightarrow> bool" where
+  "R_3  \<equiv> R_' ===> consistentS R_'"
+abbreviation R_33 :: "('a \<Rightarrow> 'b \<Rightarrow> 'c) \<Rightarrow> ('a ==_\<Longrightarrow> 'b ==_\<Longrightarrow> 'c) \<Rightarrow> bool" where
+  "R_33 \<equiv> R_' ===> consistentS R_3"
+abbreviation R_333 :: "('a \<Rightarrow> 'b \<Rightarrow> 'c \<Rightarrow> 'd) \<Rightarrow> ('a ==_\<Longrightarrow> 'b ==_\<Longrightarrow> 'c==_\<Longrightarrow> 'd) \<Rightarrow> bool" where
+  "R_333 \<equiv> R_' ===> consistentS R_33"
+abbreviation R_q3p33 :: "(('a \<Rightarrow> 'b) \<Rightarrow> 'c \<Rightarrow> 'd) \<Rightarrow> (('a ==_\<Longrightarrow> 'b) ==_\<Longrightarrow> 'c ==_\<Longrightarrow> 'd) \<Rightarrow> bool" where
+  "R_q3p33 \<equiv> R_3 ===> consistentS R_3"
+abbreviation R_q33p333 :: "(('a \<Rightarrow> 'b \<Rightarrow> 'c) \<Rightarrow> 'd \<Rightarrow> 'e \<Rightarrow> 'f) \<Rightarrow> (('a ==_\<Longrightarrow> 'b ==_\<Longrightarrow> 'c) ==_\<Longrightarrow> 'd ==_\<Longrightarrow> 'e ==_\<Longrightarrow> 'f) \<Rightarrow> bool" where
+  "R_q33p333 \<equiv> R_33 ===> consistentS R_33"
+  
 term 0 (**)
-
-definition consistentDP :: "('param \<Rightarrow> 'result) \<Rightarrow> ('param \<Rightarrow>\<^sub>T 'result) \<Rightarrow> bool" where
-  "consistentDP dp dp\<^sub>T \<equiv> \<forall>param. consistentS dp (dp param) (dp\<^sub>T param)"
+  
+definition consistentDP :: "('param \<Rightarrow>\<^sub>T 'result) \<Rightarrow> bool" where
+  "consistentDP \<equiv> R_3 dp"
 term 0 (**)
-
-(* consistentM *)
+  
+  (* consistentM *)
 lemma consistentM_intro:
   assumes "\<And>param v. M param = Some v \<Longrightarrow> v = dp param"
-  shows "consistentM dp M"
+  shows "consistentM M"
   using assms unfolding consistentM_def by blast
 term 0 (**)
-
+  
 lemma consistentM_elim:
-  assumes "consistentM dp M" "M param = Some v"
+  assumes "consistentM M" "M param = Some v"
   obtains "dp param = v"
   using assms unfolding consistentM_def dom_def by auto
 term 0 (**)
-
-(* consistentS *)
+  
+  (* consistentS *)
 lemma consistentS_intro:
-  assumes "\<And>M v' M'. \<lbrakk>consistentM dp M; runState v\<^sub>T M = (v', M')\<rbrakk> \<Longrightarrow> v = v' \<and> consistentM dp M'"
-  shows "consistentS dp v v\<^sub>T"
+  assumes "\<And>M v' M'. \<lbrakk>consistentM M; runState v\<^sub>T M = (v', M')\<rbrakk> \<Longrightarrow> R v v' \<and> consistentM M'"
+  shows "consistentS R v v\<^sub>T"
   using assms unfolding consistentS_def by blast
 term 0 (**)
-
+  
 lemma consistentS_elim:
-  assumes "consistentS dp v v\<^sub>T" "consistentM dp M"
-  obtains v' M' where "runState v\<^sub>T M = (v', M')" "v = v'" "consistentM dp M'"
+  assumes "consistentS R v v\<^sub>T" "consistentM M"
+  obtains v' M' where "runState v\<^sub>T M = (v', M')" "R v v'" "consistentM M'"
   using assms unfolding consistentS_def by blast
 term 0 (**)
-
-(* consistentS_0arg *)
-lemma consistentS_0arg_intro:
-  assumes "consistentS dp v v\<^sub>T"
-  shows "consistentS_0arg dp v v\<^sub>T"
-  using assms unfolding consistentS_0arg_def .
-term 0 (**)
-
-lemma consistentS_0arg_elim:
-  assumes "consistentS_0arg dp v v\<^sub>T"
-  obtains "consistentS dp v v\<^sub>T"
-  using assms unfolding consistentS_0arg_def ..
-term 0 (**)
-
-(*consistentS_1arg *)
-lemma consistentS_1arg_intro:
-  assumes "\<And>x. consistentS_0arg dp (f x) (f\<^sub>T . \<langle>x\<rangle>)"
-  shows "consistentS_1arg dp f f\<^sub>T"
-  using assms unfolding consistentS_1arg_def ..
-
-(* consistentDP *)
+  
+  (* consistentDP *)
 lemma consistentDP_intro:
-  assumes "\<And>param. consistentS dp (dp param) (dp\<^sub>T param)"
-  shows "consistentDP dp dp\<^sub>T"
+  assumes "\<And>param. consistentS R_' (dp param) (dp\<^sub>T param)"
+  shows "consistentDP dp\<^sub>T"
   using assms unfolding consistentDP_def by blast
 term 0 (**)
-
-(** Transfer rules **)
+  
+  (** Transfer rules **)
 lemma consistentS_return_transfer[transfer_rule]:
-  "(op = ===> consistentS dp) (\<lambda>x. x) return"
+  "(R ===> consistentS R) (\<lambda>x. x) (\<lambda>x. \<langle>x\<rangle>)"
   unfolding rel_fun_def return_def by (fastforce intro: consistentS_intro)
 lemmas consistentS_return = consistentS_return_transfer[unfolded rel_fun_def, rule_format]
 term 0 (**)
-
-(* Low level operators *)
+  
+  (* Low level operators *)
 lemma consistentM_upd:
-  assumes "consistentM dp M" "v = dp param"
-  shows "consistentM dp (M(param\<mapsto>v))"
+  assumes "consistentM M" "v = dp param"
+  shows "consistentM (M(param\<mapsto>v))"
   using assms unfolding consistentM_def by auto
 term 0 (**)
-
-lemma consistentS_get:
-  assumes "\<And>M. consistentM dp M \<Longrightarrow> consistentS dp v (sf M)"
-  shows "consistentS dp v (get \<bind> sf)"
-  using assms unfolding get_def bind_def by (fastforce intro: consistentS_intro elim: consistentS_elim split: prod.split)
   
+lemma consistentS_get:
+  assumes "\<And>M. consistentM M \<Longrightarrow> consistentS R v (sf M)"
+  shows "consistentS R v (get \<bind> sf)"
+  using assms unfolding get_def bind_def by (fastforce intro: consistentS_intro elim: consistentS_elim split: prod.split)
+    
 term 0 (**)
-
+  
 lemma consistentS_put:
-  assumes "consistentS dp v sf" "consistentM dp M"
-  shows "consistentS dp v (put M \<then> sf)"
+  assumes "consistentS R v sf" "consistentM M"
+  shows "consistentS R v (put M \<then> sf)"
   using assms unfolding put_def bind_def by (fastforce intro: consistentS_intro elim: consistentS_elim split: prod.split)
 term 0 (**)
-
-lemma consistentS_app:
-  assumes "consistentS dp v s" "consistentS dp v' (sf v)"
-  shows "consistentS dp v' (s \<bind> sf)"
-  using assms unfolding bind_def by (fastforce intro: consistentS_intro elim: consistentS_elim split: prod.split)
+  
+lemma consistentS_bind:
+  assumes "consistentS R_' v s" "consistentS R_' (f v) (sf v)"
+  shows "consistentS R_' (f v) (s \<bind> sf)"
+  using assms unfolding bind_def rel_fun_def by (fastforce intro: consistentS_intro elim: consistentS_elim split: prod.split)
 term 0 (**)
-
+  
 lemma consistentS_checkmem:
-  assumes "consistentS dp (dp param) s"
-  shows "consistentS dp (dp param) (checkmem param s)"
-  using assms unfolding checkmem_def by (fastforce intro: consistentS_return consistentS_get
-      consistentS_put consistentS_app consistentM_upd elim: consistentM_elim split: option.splits)
+  assumes "consistentS R_' (dp param) s"
+  shows "consistentS R_' (dp param) (checkmem param s)"
+  using assms unfolding checkmem_def
+  by (fastforce intro: consistentS_return consistentS_get
+      consistentS_put consistentS_bind consistentM_upd elim: consistentM_elim split: option.splits)
 term 0 (**)
+  
+lemma fun_app_lifted_transfer[transfer_rule]:
+  "(consistentS (R ===> consistentS R') ===> consistentS R ===> consistentS R') (\<lambda>f x. f x) (\<lambda>f\<^sub>T x\<^sub>T. f\<^sub>T . x\<^sub>T)"
+proof -
+  { fix f f\<^sub>T x x\<^sub>T assume sf: "consistentS (R ===> consistentS R') f f\<^sub>T" and sx: "consistentS R x x\<^sub>T"
+    { fix M ov oM assume cm: "consistentM M" and os:"runState (f\<^sub>T . x\<^sub>T) M = (ov, oM)"
+      obtain fv M' where bf: "runState f\<^sub>T M = (fv, M')" and rf: "(R ===> consistentS R') f fv" and cm':"consistentM M'"
+        using sf cm by (auto elim: consistentS_elim)
+      obtain xv M'' where bx: "runState x\<^sub>T M' = (xv, M'')" and rx: "R x xv" and cm'': "consistentM M''"
+        using sx cm' by (auto elim: consistentS_elim)
+      have srfx: "consistentS R' (f x) (fv xv)"
+        using rf rx by (auto dest: rel_funD)
+      obtain res M''' where bres: "runState (fv xv) M'' = (res, M''')" and rres: "R' (f x) (res)" and cm''': "consistentM M'''"
+        using srfx cm'' by (auto elim: consistentS_elim)
+      have bfx: "runState (f\<^sub>T . x\<^sub>T) M = (res, M''')"
+        unfolding fun_app_lifted_def bind_def by (auto simp: bf bx bres)
+      have "R' (f x) ov" "consistentM oM"
+        using os bfx rres cm''' by auto
+    } hence "consistentS R' (f x) (f\<^sub>T . x\<^sub>T)" by (blast intro: consistentS_intro)
+  } thus ?thesis by blast
+qed
 
+lemma lift_'_transfer[transfer_rule]: "R_' x (lift_' x)"
+  unfolding lift_'_def ..
+
+lemma lift_3_transfer[transfer_rule]: "R_3 f (lift_3 f)"
+  unfolding lift_3_def lift_'_def by transfer_prover
+
+lemma lift_33_transfer[transfer_rule]: "R_33 f (lift_33 f)"
+  unfolding lift_33_def lift_3_def lift_'_def by transfer_prover
+term 0 (**)
+  
+lemma lift_Cons_transfer[transfer_rule]: "R_33 Cons Cons\<^sub>T"
+  unfolding Cons\<^sub>T_def by transfer_prover
+
+term 0 (**)
+lemma "R_q3p33 map map\<^sub>T"
+proof -
+  fix f f\<^sub>T assume "R_3 f f\<^sub>T"
+  have "consistentS R_' (map f xs) (map\<^sub>T' f\<^sub>T xs)" for xs
+    apply (induction xs)
+     apply (unfold list.map map\<^sub>T'.simps)
+    subgoal by transfer_prover
+    subgoal premises prems thm prems
+      apply transfer_prover_start
+                  prefer 8 apply transfer_step
+                 prefer 5 apply transfer_step
+                prefer 6 apply transfer_step
+               prefer 7 apply transfer_step
+              prefer 7 apply transfer_step
+             prefer 7 apply transfer_step
+            prefer 6 apply transfer_step
+           apply transfer_step
+          apply transfer_step
+      term lfp
+      oops
 end
-
+end
 end
