DP_Lifting.thy
@@ -1,17 +1,22 @@
 theory DP_Lifting
   imports Main "./Monad"
 begin
-
-(* Types *)
+  
+  (* Types *)
 type_synonym ('a,'M,'b) fun_lifted = "'a \<Rightarrow> ('M,'b) state" ("_ ==_\<Longrightarrow> _" [3,1000,2] 2)
 type_synonym ('a,'b) dpfun = "'a ==('a\<rightharpoonup>'b)\<Longrightarrow> 'b" (infixr "\<Rightarrow>\<^sub>T" 2)
 term 0 (**)
-
-(* Basics *)
+  
+  (* Basics *)
 definition fun_app_lifted :: "('M,'a =='M\<Longrightarrow> 'b) state \<Rightarrow> ('M,'a) state \<Rightarrow> ('M,'b) state" (infixl "." 999) where
   "f\<^sub>T . x\<^sub>T \<equiv> do { f \<leftarrow> f\<^sub>T; x \<leftarrow> x\<^sub>T; f x }"
+  
+lemma fun_app_lifted_elim:
+  assumes "runState (f\<^sub>T . x\<^sub>T) M = (v, Mv)" "runState f\<^sub>T M = (f, Mf)"
+  obtains x Mx where "runState x\<^sub>T Mf = (x, Mx)" and "runState (f x) Mx = (v, Mv)"
+  using assms unfolding fun_app_lifted_def bind_def by (auto split: prod.splits)
 term 0 (**)
-
+  
 definition checkmem :: "'param \<Rightarrow> ('param \<rightharpoonup> 'result, 'result) state \<Rightarrow> ('param \<rightharpoonup> 'result, 'result) state" where
   "checkmem param calc \<equiv> do {
     M \<leftarrow> get;
@@ -24,95 +29,95 @@ definition checkmem :: "'param \<Rightarrow> ('param \<rightharpoonup> 'result, 
         \<langle>x\<rangle>
       }
   }"
-
+  
 abbreviation checkmem_eq :: "('param \<Rightarrow>\<^sub>T 'result) \<Rightarrow> 'param \<Rightarrow> ('param \<rightharpoonup> 'result, 'result) state \<Rightarrow> bool" ("_$ _ =CHECKMEM= _" [1000,51] 51) where
   "(dp\<^sub>T$ param =CHECKMEM= calc) \<equiv> (dp\<^sub>T param = checkmem param calc)"
 term 0 (**)
-
-(* Auxiliary *)
-definition lift_0arg :: "'a \<Rightarrow> 'a" where
-  "lift_0arg x \<equiv> x"
-definition lift_1arg :: "('a \<Rightarrow> 'b) \<Rightarrow> ('a =='M\<Longrightarrow> 'b)" where
-  "lift_1arg f \<equiv> \<lambda>v. \<langle>lift_0arg (f v)\<rangle>"
-definition lift_2arg :: "('a \<Rightarrow> 'b \<Rightarrow> 'c) \<Rightarrow> ('a =='M\<Longrightarrow> 'b =='M\<Longrightarrow> 'c)" where
-  "lift_2arg f \<equiv> \<lambda>v. \<langle>lift_1arg (f v)\<rangle>"
-definition lift_3arg :: "('a \<Rightarrow> 'b \<Rightarrow> 'c \<Rightarrow> 'd) \<Rightarrow> ('a =='M\<Longrightarrow> 'b =='M\<Longrightarrow> 'c =='M\<Longrightarrow> 'd)" where
-  "lift_3arg f \<equiv> \<lambda>v. \<langle>lift_2arg (f v)\<rangle>"
-
+  
+  (* Auxiliary *)
+definition lift_' :: "'a \<Rightarrow> 'a" where
+  "lift_' x \<equiv> x"
+definition lift_3 :: "('a \<Rightarrow> 'b) \<Rightarrow> ('a =='M\<Longrightarrow> 'b)" where
+  "lift_3 f \<equiv> \<lambda>v. \<langle>lift_' (f v)\<rangle>"
+definition lift_33 :: "('a \<Rightarrow> 'b \<Rightarrow> 'c) \<Rightarrow> ('a =='M\<Longrightarrow> 'b =='M\<Longrightarrow> 'c)" where
+  "lift_33 f \<equiv> \<lambda>v. \<langle>lift_3 (f v)\<rangle>"
+definition lift_333 :: "('a \<Rightarrow> 'b \<Rightarrow> 'c \<Rightarrow> 'd) \<Rightarrow> ('a =='M\<Longrightarrow> 'b =='M\<Longrightarrow> 'c =='M\<Longrightarrow> 'd)" where
+  "lift_333 f \<equiv> \<lambda>v. \<langle>lift_33 (f v)\<rangle>"
+  
 definition unlift_0arg :: "('M, 'a) state \<Rightarrow> ('M, 'a) state" where
   "unlift_0arg x\<^sub>T \<equiv> x\<^sub>T"
 definition unlift_1arg :: "('M, 'a =='M\<Longrightarrow> 'b) state \<Rightarrow> ('a \<Rightarrow> ('M, 'b) state)" where
   "unlift_1arg f\<^sub>T \<equiv> \<lambda>v. unlift_0arg (f\<^sub>T . \<langle>v\<rangle>)"
 definition unlift_2arg :: "('M, 'a =='M\<Longrightarrow> 'b =='M\<Longrightarrow> 'c) state \<Rightarrow> ('a \<Rightarrow> 'b \<Rightarrow> ('M, 'c) state)" where
   "unlift_2arg f\<^sub>T \<equiv> \<lambda>v. unlift_1arg (f\<^sub>T . \<langle>v\<rangle>)"
-
+  
 term 0 (**)
-
-(* HOL *)
+  
+  (* HOL *)
 definition If\<^sub>T :: "bool =='M\<Longrightarrow> 'a =='M\<Longrightarrow> 'a =='M\<Longrightarrow> 'a" where
-  "If\<^sub>T \<equiv> lift_3arg If"
-
+  "If\<^sub>T \<equiv> lift_333 If"
+  
 thm fcomp_def
 definition fcomp\<^sub>T :: "('b =='M\<Longrightarrow> 'c) =='M\<Longrightarrow> ('a =='M\<Longrightarrow> 'b) =='M\<Longrightarrow> ('a =='M\<Longrightarrow> 'c)" where
   "fcomp\<^sub>T \<equiv> \<lambda>g. \<langle>\<lambda>f. \<langle>\<lambda>x. \<langle>g\<rangle> . (\<langle>f\<rangle>.\<langle>x\<rangle>) \<rangle>\<rangle>"
-
+  
 definition id\<^sub>T :: "'a =='M\<Longrightarrow> 'a" where
   "id\<^sub>T \<equiv> \<lambda>x. \<langle>x\<rangle>"
 term 0 (**)
-
-(* List *)
+  
+  (* List *)
 definition Cons\<^sub>T :: "'a =='M\<Longrightarrow> 'a list =='M\<Longrightarrow> 'a list" where
-  "Cons\<^sub>T \<equiv> lift_2arg Cons"
-
+  "Cons\<^sub>T \<equiv> lift_33 Cons"
+  
 definition case_list\<^sub>T :: "'b =='M\<Longrightarrow> ('a =='M\<Longrightarrow> 'a list =='M\<Longrightarrow> 'b) =='M\<Longrightarrow> 'a list =='M\<Longrightarrow> 'b" where
   "case_list\<^sub>T \<equiv> \<lambda>ifNil. \<langle>\<lambda>ifCons. \<langle>\<lambda>val. case_list (unlift_0arg \<langle>ifNil\<rangle>) (unlift_2arg \<langle>ifCons\<rangle>) val\<rangle>\<rangle>"
-
+  
 primrec map\<^sub>T' :: "('a =='M\<Longrightarrow>'b) \<Rightarrow> 'a list =='M\<Longrightarrow> 'b list" where
   "(map\<^sub>T' f) [] = \<langle>[]\<rangle>"
 | "(map\<^sub>T' f) (x#xs) = \<langle>Cons\<^sub>T\<rangle> . (\<langle>f\<rangle> . \<langle>x\<rangle>) . ((map\<^sub>T' f) xs)"
 lemma
   "(map\<^sub>T' f) (x#xs) = \<langle>Cons\<^sub>T\<rangle> . (\<langle>f\<rangle> . \<langle>x\<rangle>) . (\<langle>map\<^sub>T' f\<rangle> . \<langle>xs\<rangle>)" unfolding map\<^sub>T'.simps(2) fun_app_lifted_def left_identity ..
-
+    
 definition map\<^sub>T :: "('a =='M\<Longrightarrow> 'b) =='M\<Longrightarrow> 'a list =='M\<Longrightarrow> 'b list" where
-  "map\<^sub>T \<equiv> lift_1arg map\<^sub>T'"
-
+  "map\<^sub>T \<equiv> lift_3 map\<^sub>T'"
+  
 primrec fold\<^sub>T' :: "('a =='M\<Longrightarrow> 'b =='M\<Longrightarrow> 'b) \<Rightarrow> 'a list =='M\<Longrightarrow> 'b =='M\<Longrightarrow> 'b" where
   "(fold\<^sub>T' f) [] = \<langle>id\<^sub>T\<rangle>"
 | "(fold\<^sub>T' f) (x#xs) = \<langle>fcomp\<^sub>T\<rangle> . (\<langle>f\<rangle> . \<langle>x\<rangle>) . ((fold\<^sub>T' f) xs)"
 lemma
   "(fold\<^sub>T' f) (x#xs) = \<langle>fcomp\<^sub>T\<rangle> . (\<langle>f\<rangle> . \<langle>x\<rangle>) . (\<langle>fold\<^sub>T' f\<rangle> . \<langle>xs\<rangle>)" unfolding fold\<^sub>T'.simps(2) fun_app_lifted_def left_identity ..
-
+    
 definition fold\<^sub>T :: "('a =='M\<Longrightarrow> 'b =='M\<Longrightarrow> 'b) =='M\<Longrightarrow> 'a list =='M\<Longrightarrow> 'b =='M\<Longrightarrow> 'b" where
-  "fold\<^sub>T \<equiv> lift_1arg fold\<^sub>T'"
-
+  "fold\<^sub>T \<equiv> lift_3 fold\<^sub>T'"
+  
 term 0 (**)
-
-(* Option *)
+  
+  (* Option *)
 definition Some\<^sub>T :: "'a =='M\<Longrightarrow> 'a option" where
-  "Some\<^sub>T \<equiv> lift_1arg Some"
-
+  "Some\<^sub>T \<equiv> lift_3 Some"
+  
 definition case_option\<^sub>T :: "'b =='M\<Longrightarrow> ('a =='M\<Longrightarrow> 'b) =='M\<Longrightarrow> 'a option =='M\<Longrightarrow> 'b" where
   "case_option\<^sub>T \<equiv> \<lambda>ifNone. \<langle>\<lambda>ifSome. \<langle>\<lambda>val. case_option (unlift_0arg \<langle>ifNone\<rangle>) (unlift_1arg \<langle>ifSome\<rangle>) val\<rangle>\<rangle>"
 term 0 (**)
-
-(* Prod *)
+  
+  (* Prod *)
 definition Pair\<^sub>T :: "'a0 =='M\<Longrightarrow> 'a1 =='M\<Longrightarrow> 'a0\<times>'a1" where
-  "Pair\<^sub>T \<equiv> lift_2arg Pair"
-
+  "Pair\<^sub>T \<equiv> lift_33 Pair"
+  
 definition case_prod\<^sub>T :: "('a0 =='M\<Longrightarrow> 'a1 =='M\<Longrightarrow> 'b) =='M\<Longrightarrow> ('a0\<times>'a1) =='M\<Longrightarrow> 'b" where
   "case_prod\<^sub>T \<equiv> \<lambda>ifProd. \<langle>\<lambda>val. case_prod (unlift_2arg \<langle>ifProd\<rangle>) val\<rangle>"
-
+  
 term "\<langle>case_prod\<^sub>T\<rangle> . \<langle>\<lambda>v0. \<langle>\<lambda>v1. \<langle>v0+v1\<rangle>\<rangle>\<rangle> . (\<langle>Pair\<^sub>T\<rangle> . \<langle>0\<rangle> . \<langle>0::int\<rangle>)"
 term 0 (**)
-
-(* Arithmetic *)
+  
+  (* Arithmetic *)
 definition min\<^sub>T :: "'a::ord =='M\<Longrightarrow> 'a =='M\<Longrightarrow> 'a" where
-  "min\<^sub>T \<equiv> lift_2arg min"
-
+  "min\<^sub>T \<equiv> lift_33 min"
+  
 definition max\<^sub>T :: "'a::ord =='M\<Longrightarrow> 'a =='M\<Longrightarrow> 'a" where
-  "max\<^sub>T \<equiv> lift_2arg max"
-
+  "max\<^sub>T \<equiv> lift_33 max"
+  
 definition plus\<^sub>T :: "'a::plus =='M\<Longrightarrow> 'a =='M\<Longrightarrow> 'a" where
-  "plus\<^sub>T \<equiv> lift_2arg plus"
+  "plus\<^sub>T \<equiv> lift_33 plus"
 term 0 (**)
 end
